\documentclass{article}

\usepackage{amsmath}
\usepackage{amssymb}
\usepackage{amsthm}

\addtolength{\oddsidemargin}{-.575in}
\addtolength{\evensidemargin}{-.575in}
\addtolength{\textwidth}{1.0in}
\addtolength{\topmargin}{-.575in}
\addtolength{\textheight}{1.25in}

\newcommand{\R}{\mathbb{R}}
\newcommand{\V}{\mathbb{V}}
\newcommand{\G}{\mathbb{G}}
\newcommand{\prl}{\parallel}
\newcommand{\prp}{\perp}
\newcommand{\nlo}{o}
\newcommand{\nli}{\infty}

%\swapnumbers
\newtheorem{theorem}{Theorem}[section]
\newtheorem{definition}{Definition}[section]
\newtheorem{corollary}{Corollary}[section]
\newtheorem{identity}{Identity}[section]

\title{A Problem For Paul}
%\author{Spencer T. Parkin}

\begin{document}
\maketitle

\section*{The Problem}

Given a 2-blade $B$ and a vector $v$, find the vector $v'$ which is the orthogonal
reflection of $v$ about $B$.

\section*{One Possible Solution}

Start by drawing a picture!

Now, without loss of generality, we can write $B$ as
\begin{equation*}
B = a\wedge b,
\end{equation*}
where $a$ and $b$ are a pair of orthogonal vectors, where $b$ is unit-length, and where $v$ is orthogonal to the vector $a$.

It follows that $|a|=|B|$.  Why?

We will now prove that
\begin{equation*}
v' = -BvB^{-1}.
\end{equation*}

To begin, notice that $B = ab$.  Why?

Next, notice that $B^{-1}=ba/|a|^2$.  Why?

We then notice that $bvb = v'$.  Why?

Now notice that $-av'a/|a|^2=v'$.  Why?

We now see that
\begin{equation*}
-BvB^{-1} = -\frac{abvba}{|a|^2} = -\frac{av'a}{|a|^2} = v'.
\end{equation*}
And there we have it!

\section*{Another Possible Solution}

Notice that $v_{\parallel}=(v\cdot B)B^{-1}$ and $v_{\perp}=(v\wedge B)B^{-1}$.  We then have
\begin{align*}
v' &= a_{\parallel} - a_{\perp} \\
 &= (a\cdot B)B^{-1} - (a\wedge B)B^{-1} \\
 &= -(B\cdot a)B^{-1} - (B\wedge a)B^{-1} \\
 &= -(B\cdot a + B\wedge a)B^{-1} \\
 &= -BaB^{-1},
\end{align*}
which confirms the earlier result!

\end{document}